refactor even more rotation 64

Clean/Gadgets/Rotation64/Rotation64.lean
@@ -2,7 +2,7 @@ import Clean.Types.U64
 import Clean.Circuit.SubCircuit
 import Clean.Gadgets.Rotation64.Theorems
 import Clean.Gadgets.Rotation64.Rotation64Bytes
-import Clean.Gadgets.Rotation64.ByteRotationTable
+import Clean.Gadgets.Rotation64.Rotation64Bits
 import Clean.Gadgets.ByteDecomposition
 import Clean.Circuit.Provable
 
@@ -22,29 +22,12 @@ open Gadgets.Rotation64 (byte_rotation_lookup)
   Rotate the 64-bit integer by `offset` bits
 -/
 def rot64 (offset : Fin 64) (x : Var U64 (F p)) : Circuit (F p) (Var U64 (F p)) := do
-  let byte_offset := offset / 8
+  let byte_offset : ℕ := offset.val / 8
   let bit_offset : ℕ := (offset % 8).val
 
-  -- apply the bit rotation
-  let ⟨low, high⟩ ← subcircuit (Gadgets.U64ByteDecomposition.circuit bit_offset) x
-  let ⟨x0_l, x1_l, x2_l, x3_l, x4_l, x5_l, x6_l, x7_l⟩ := low
-  let ⟨x0_h, x1_h, x2_h, x3_h, x4_h, x5_h, x6_h, x7_h⟩ := high
-
-  let ⟨y0, y1, y2, y3, y4, y5, y6, y7⟩ ← U64.witness fun _env => U64.mk 0 0 0 0 0 0 0 0
-
-  assert_zero (x1_l * ((2 : ℕ)^(8 - bit_offset) : F p) + x0_h - y0)
-  assert_zero (x2_l * ((2 : ℕ)^(8 - bit_offset) : F p) + x1_h - y1)
-  assert_zero (x3_l * ((2 : ℕ)^(8 - bit_offset) : F p) + x2_h - y2)
-  assert_zero (x4_l * ((2 : ℕ)^(8 - bit_offset) : F p) + x3_h - y3)
-  assert_zero (x5_l * ((2 : ℕ)^(8 - bit_offset) : F p) + x4_h - y4)
-  assert_zero (x6_l * ((2 : ℕ)^(8 - bit_offset) : F p) + x5_h - y5)
-  assert_zero (x7_l * ((2 : ℕ)^(8 - bit_offset) : F p) + x6_h - y6)
-  assert_zero (x0_l * ((2 : ℕ)^(8 - bit_offset) : F p) + x7_h - y7)
-
-  -- apply the byte rotation
-  let y ← subcircuit (Gadgets.Rotation64Bytes.circuit byte_offset) ⟨y0, y1, y2, y3, y4, y5, y6, y7⟩
-  let out ← U64.copy y
-  return out
+  -- rotation is performed by combining a bit and a byte rotation
+  let byte_rotated ← subcircuit (Rotation64Bytes.circuit byte_offset) x
+  subcircuit (Rotation64Bits.circuit bit_offset) byte_rotated
 
 instance lawful (off : Fin 64) : ConstantLawfulCircuits (F := (F p)) (rot64 off) := by infer_constant_lawful_circuits
 
@@ -58,8 +41,8 @@ def spec (offset : Fin 64) (x : U64 (F p)) (y: U64 (F p)) :=
 #eval! (rot64 (p:=p_babybear) 0) default |>.output
 def elaborated (off : Fin 64) : ElaboratedCircuit (F p) U64 (Var U64 (F p)) where
   main := rot64 off
-  local_length _ := 32
-  output _inputs i0 := var_from_offset U64 (i0 + 24)
+  local_length _ := 24
+  output _inputs i0 := var_from_offset U64 (i0 + 16)
   initial_offset_eq := by
     intros
     simp only [rot64]
@@ -71,11 +54,8 @@ def elaborated (off : Fin 64) : ElaboratedCircuit (F p) U64 (Var U64 (F p)) wher
 
 
 theorem soundness (offset : Fin 64) : Soundness (F p) (circuit := elaborated offset) assumptions (spec offset) := by
-  intro i0 env ⟨x0_var, x1_var, x2_var, x3_var, x4_var, x5_var, x6_var, x7_var ⟩ ⟨x0, x1, x2, x3, x4, x5, x6, x7⟩ h_input x_byte h_holds
+  intro i0 env ⟨x0_var, x1_var, x2_var, x3_var, x4_var, x5_var, x6_var, x7_var ⟩ ⟨x0, x1, x2, x3, x4, x5, x6, x7⟩ h_input x_normalized h_holds
 
-  simp [elaborated, subcircuit_norm, rot64, Circuit.constraints_hold.soundness, U64.witness] at h_holds
-  -- simp [circuit_norm, subcircuit_norm, U64ByteDecomposition.circuit, U64ByteDecomposition.elaborated,
-  -- Rotation64Bytes.circuit, Rotation64Bytes.elaborated] at h_holds
   sorry
 
 theorem completeness (offset : Fin 64) : Completeness (F p) (circuit := elaborated offset) U64 assumptions := by
