Clean/Gadgets/Rotation64/Rotation64Bits.lean
@@ -1,0 +1,95 @@
+import Clean.Types.U64
+import Clean.Circuit.SubCircuit
+import Clean.Gadgets.Rotation64.Theorems
+import Clean.Gadgets.Rotation64.Rotation64Bytes
+import Clean.Gadgets.Rotation64.ByteRotationTable
+import Clean.Gadgets.ByteDecomposition
+import Clean.Circuit.Provable
+
+namespace Gadgets.Rotation64Bits
+variable {p : ℕ} [Fact p.Prime]
+variable [p_large_enough: Fact (p > 2^16 + 2^8)]
+
+instance : Fact (p > 512) := by
+  constructor
+  linarith [p_large_enough.elim]
+
+open Gadgets.Rotation64.Theorems (rot_right64)
+
+/--
+  Rotate the 64-bit integer by `offset` bits
+-/
+def rot64_bits (offset : Fin 8) (x : Var U64 (F p)) : Circuit (F p) (Var U64 (F p)) := do
+
+  let two_power : F p := 2^offset.val
+
+  let ⟨low, high⟩ ← subcircuit (Gadgets.U64ByteDecomposition.circuit offset) x
+  let ⟨x0_l, x1_l, x2_l, x3_l, x4_l, x5_l, x6_l, x7_l⟩ := low
+  let ⟨x0_h, x1_h, x2_h, x3_h, x4_h, x5_h, x6_h, x7_h⟩ := high
+
+  let ⟨y0, y1, y2, y3, y4, y5, y6, y7⟩ ← U64.witness fun _env => U64.mk 0 0 0 0 0 0 0 0
+
+  assert_zero (x1_l * two_power + x0_h - y0)
+  assert_zero (x2_l * two_power + x1_h - y1)
+  assert_zero (x3_l * two_power + x2_h - y2)
+  assert_zero (x4_l * two_power + x3_h - y3)
+  assert_zero (x5_l * two_power + x4_h - y4)
+  assert_zero (x6_l * two_power + x5_h - y5)
+  assert_zero (x7_l * two_power + x6_h - y6)
+  assert_zero (x0_l * two_power + x7_h - y7)
+  return ⟨y0, y1, y2, y3, y4, y5, y6, y7⟩
+
+instance lawful (off : Fin 8) : ConstantLawfulCircuits (F := (F p)) (rot64_bits off) := by infer_constant_lawful_circuits
+
+def assumptions (input : U64 (F p)) := input.is_normalized
+
+def spec (offset : Fin 8) (x : U64 (F p)) (y: U64 (F p)) :=
+  y.value = rot_right64 x.value offset.val
+  ∧ y.is_normalized
+
+-- #eval! (rot64_bits (p:=p_babybear) 0) default |>.operations.local_length
+-- #eval! (rot64_bits (p:=p_babybear) 0) default |>.output
+def elaborated (off : Fin 8) : ElaboratedCircuit (F p) U64 (Var U64 (F p)) where
+  main := rot64_bits off
+  local_length _ := 24
+  output _inputs i0 := var_from_offset U64 (i0 + 16)
+  initial_offset_eq := by
+    intros
+    simp only [rot64_bits]
+    rfl
+  local_length_eq := by
+    intros
+    simp only [rot64_bits]
+    rfl
+
+set_option maxHeartbeats 10000000
+theorem soundness (offset : Fin 8) : Soundness (F p) (circuit := elaborated offset) assumptions (spec offset) := by
+  intro i0 env ⟨x0_var, x1_var, x2_var, x3_var, x4_var, x5_var, x6_var, x7_var ⟩ ⟨x0, x1, x2, x3, x4, x5, x6, x7⟩ h_input x_normalized h_holds
+
+  -- TODO: this is slow
+  simp [circuit_norm, elaborated, rot64_bits, U64.witness] at h_holds
+  simp [subcircuit_norm, U64.AssertNormalized.assumptions, U64.AssertNormalized.circuit, circuit_norm] at h_holds
+  save
+
+  simp [U64ByteDecomposition.circuit, U64ByteDecomposition.elaborated, U64ByteDecomposition.spec,
+    U64ByteDecomposition.assumptions, U64.AssertNormalized.spec, circuit_norm, eval] at h_holds
+
+  save
+
+  simp [circuit_norm, spec, rot_right64, eval, elaborated]
+  -- now the statement is reasonable
+
+  sorry
+
+theorem completeness (offset : Fin 8) : Completeness (F p) (circuit := elaborated offset) U64 assumptions := by
+  sorry
+
+def circuit (offset : Fin 8) : FormalCircuit (F p) U64 U64 := {
+  elaborated offset with
+  assumptions := assumptions
+  spec := spec offset
+  soundness := soundness offset
+  completeness := completeness offset
+}
+
+end Gadgets.Rotation64Bits
